Dafny/Common/SameDifferenece.i.dfy
@@ -1,0 +1,217 @@
+
+include "../LLVM/ops.dfy"
+include "../LLVM/types.dfy"
+include "../Libraries/Seqs.s.dfy"
+include "../Libraries/Seqs.i.dfy"
+
+
+// // Old      |   New
+// // x := 0   |   x := 0
+// // s0       |   s0
+// // z := 0   |   z := 1
+// // s        |   p
+// // y := x   |   y := x
+// // s'       |   p'
+// function ExecuteOneInst(s, s') {
+//   // Represents the difference between s, s' after executing instruction s.pc
+//   // For example: ExecuteOneInst(s, s') == ExecuteOneInst(p, p') == UpdateStmt(y, x)
+// }
+// predicate NextSameDiff(s, s', p, p')
+// {
+//   && s.pc == p.pc       // Maybe something more sophisticated here to describe s.pc and p.pc also map to the same instruction
+//   && ExecuteOneInst(s, s') == ExecuteOneInst(p, p')
+// }
+
+module AbstractSameDifference {
+    import opened types
+    import opened ops
+    import opened Collections__Seqs_s
+    import opened Collections__Seqs_i
+
+    type name = string
+
+    datatype state = State(
+        vals:map<name, int>,
+        pc:int,
+        ok:bool)
+
+    type behavior = seq<state>
+
+
+    datatype codeRe =
+    | Ins(ins:ins)
+    | Block(block:codeSeq)
+    | IfElse(ifCond:int, ifTrue:codeSeq, ifFalse:codeSeq)
+    | Divergence(pre:codeSeq,post:codeSeq,patched:bool)
+    | NonImpactIns(NIIns:ins)
+    | CNil
+
+     datatype ins =
+    | ADD(dst:int, size:nat, src1ADD:int, src2ADD:int)
+    | SUB(dst:int, size:nat, src1SUB:int, src2SUB:int)
+    | ICMP(dst:int,cond:condition,size:nat,src1:int,src2:int)
+
+    // datatype int = D(d:Data) | LV(l:LocalVar) | GV(g:GlobalVar)
+    type codeSeq = seq<codeRe>
+
+    type simpleCode = seq<stateVal>
+
+    datatype stateVal = Val(n:name,i:int) | Nil  
+    
+    
+    predicate ValidState(s:state)
+    {
+        s.ok
+    }
+
+    datatype Step =
+        | updateStep(sv:stateVal) 
+        | updateStepNonImpact(sv:stateVal) 
+        | stutterStep()
+
+    predicate NextStep(s:state, s':state, step:Step)
+    {
+        match step  
+            case updateStep(sv) => sv.Val? && s' == updateVal(s,sv.n,sv.i) && s'.pc == s.pc+1
+            case updateStepNonImpact(sv) => sv.Val? && s' == updateVal(s,sv.n,sv.i) && s'.pc == s.pc+1
+            case stutterStep() => stutter(s,s')
+    }
+
+    predicate StateNext(s:state,s':state)
+    {
+        && exists step :: NextStep(s,s',step)
+        && ValidState(s)
+    
+    }
+
+    predicate stutter(s:state,s':state)
+    {
+        s == s'
+    }
+    
+    predicate errorStep(s:state,s':state)
+    {
+        ValidState(s) && !s'.ok
+    }
+
+    predicate ValidBehavior(states:behavior)
+    {
+        || |states| == 0
+        || (|states| == 1 && ValidState(states[0])) 
+        || (&& |states| >= 2
+            && forall s :: s in states ==> ValidState(s)
+            && forall i :: 0 <= i < |states|- 1 ==> StateNext(states[i],states[i+1]))
+    }
+
+    function evalCode(c:simpleCode, s:state) : (b:behavior)
+        
+        decreases c, 0
+    {
+        // [s]
+        if |c| == 0 then    
+            []
+        else 
+            match first(c)
+                case Nil => [s] + evalCode(all_but_first(c),s)
+                case Val(n,i) =>  [updateVal(s,n,i)] + evalCode(all_but_first(c),updateVal(s,n,i))
+                case ValNonImpact(n,i) => [updateVal(s,n,i)] + evalCode(all_but_first(c),updateVal(s,n,i))
+    
+    }
+
+
+
+
+    function updateVal(s:state,n:name,val:int) : (s':state)
+        ensures s.ok ==> s'.ok
+    {
+        var s' := s.(vals := s.vals[n := val]);
+        s'
+    }
+
+    function ExecuteOneInst(s:state, s':state,step:Step) : (sv:stateVal)
+        requires NextStep(s,s',step)
+        ensures !step.stutterStep? ==> step.sv == sv
+        // ensures step.updateStepNonImpact? ==> 
+    {
+        // assume false;
+        if step.stutterStep? then
+            var sv := Nil;
+            sv
+        else
+            assert (step.updateStep? || step.updateStepNonImpact?);
+            assert s != s';
+            var sv:stateVal :| sv.Val? && updateVal(s,sv.n,sv.i) == s';
+            assert sv.n == step.sv.n;
+            sv 
+    }
+
+    predicate NextSameDiff(s:state, s':state, p:state, p':state, step:Step)
+    {
+        && NextStep(s,s',step)
+        && NextStep(p,p',step)
+        && s.pc == p.pc       
+        && ExecuteOneInst(s, s',step) == ExecuteOneInst(p, p',step)
+    }
+
+    lemma updateStepNonImpactImpliesNextSameDiff(s:state,p:state, nonDepenStep:Step)
+        requires s.pc == p.pc  
+        requires ValidState(s);
+        requires ValidState(p);
+        requires nonDepenStep.updateStepNonImpact?
+        requires nonDepenStep.sv.Val?
+        
+        ensures forall s',p' :: (NextStep(s,s',nonDepenStep) &&  NextStep(p,p',nonDepenStep)) ==> NextSameDiff(s,s',p,p',nonDepenStep);
+    {
+
+        forall s',p' | && s' == updateVal(s,nonDepenStep.sv.n,nonDepenStep.sv.i) 
+                       && p' == updateVal(p,nonDepenStep.sv.n,nonDepenStep.sv.i)
+                       && s'.pc == s.pc + 1
+                       && p'.pc == p.pc + 1
+        ensures ExecuteOneInst(s, s',nonDepenStep) == ExecuteOneInst(p, p',nonDepenStep);
+        ensures NextSameDiff(s,s',p,p',nonDepenStep);
+        {
+            
+             assert nonDepenStep.updateStepNonImpact?;
+             assert ExecuteOneInst(s,s',nonDepenStep).Val?;
+             assert ExecuteOneInst(s, s',nonDepenStep) == ExecuteOneInst(p, p',nonDepenStep);
+             assert NextSameDiff(s,s',p,p',nonDepenStep);
+        }
+
+    }
+
+    
+
+    lemma subSeqOfBehaviorNextSameDiffIsBenign(b_s:behavior,subB_s:behavior,b_p:behavior,subB_p:behavior)
+        requires isSubSeq(b_s,subB_s)
+        requires ValidBehavior(b_s)
+        requires ValidBehavior(subB_s)
+
+        requires isSubSeq(b_p,subB_p)
+        requires ValidBehavior(b_p)
+        requires ValidBehavior(subB_p)
+
+        requires |subB_s| == |subB_p|
+        requires |subB_s| > 0;
+        requires |b_p| >= (FindIndexInSeq(b_p,first(subB_p)) + |subB_p|-1)
+        requires forall i,step_s,step_p :: && (0 <= i < |subB_p|- 1) 
+                                           && NextStep(subB_s[i], subB_s[i+1], step_s)
+                                           && NextStep(subB_p[i], subB_p[i+1], step_p)  ==> step_s == step_p
+                                     
+        requires forall i,step :: && (0 <= i < |subB_p|- 1) 
+                                  && NextStep(subB_s[i], subB_s[i+1], step)
+                                  && NextStep(subB_p[i], subB_p[i+1], step)  ==> step.updateStepNonImpact?
+    {
+
+        var first_index := FindIndexInSeq(b_p,first(subB_p));
+        assume (|b_p| >= (first_index + (|subB_p|-1)));
+
+        // assume IsBenign(b_p[first_index..first_index+|subB_p|]);
+    }
+
+    lemma patchIsBenign(c:simpleCode,patched:bool)
+        // ensures forall s :: ValidState(s) ==> IsBenign(evalCode(c,s))
+    {
+
+    }
+
+}
