Dafny/examples/simpleBenign/BenignCodeFull.s.dfy
@@ -1,0 +1,233 @@
+include "../../LLVM/llvmREFACTOR_Multi.i.dfy"
+include "../../LLVM/types.dfy"
+include "../../LLVM/control_flow.i.dfy"
+include "../../LLVM/behaviorLemmas.i.dfy"
+include "../../Libraries/Seqs.s.dfy"
+include "../../LLVM/memory.i.dfy"
+
+module simpleBenignCodeFull{
+    import opened control_flow
+    import opened LLVM_defRE_Multi
+    import opened types
+    import opened Collections__Seqs_s
+    import opened behavior_lemmas
+    import opened memory
+
+    
+
+    /////////////////////////////////////////////////////////////////////////
+
+
+    function return_():codeRe
+    {
+        var return_ := Block([Ins(RET(D(Void)))]);
+
+        return_
+    }
+
+    // function if_end4():codeRe
+    // {
+
+    //      var if_end4 := Block([Ins(LOAD(var_s,4,var_x)),
+    //                            Ins(CALL(D(Void),printf_code(global_str1()).block)),
+    //                           return_()]);
+
+    //         if_end4
+    // }
+
+    // function if_then3():codeRe
+    // {
+    //     var if_end4 := Block([Ins(LOAD(var_s,4,var_x)),
+    //                            Ins(CALL(D(Void),printf_code(global_str1()).block)),
+    //                           return_()]);
+
+    //     // var if_then3 := Block([Ins(CALL(D(Void),printf_code(global_str()).block)),
+    //     //                        Ins(UNCONDBR(if_end4()))]);
+    //     var if_then3 := Block([Ins(CALL(D(Void),printf_code(global_str()).block)),
+    //                            if_end4]);
+
+    //         if_then3
+    // }
+
+    // function benign_patch_SOI(s:state):codeRe
+    //     requires SOI_ASSIMPTIONS(s)
+    // {   
+
+    //     var var_cmp2 := LV(" var_cmp2 ");
+    //     var var_0:operand :| var_0.LV? && var_0.l in s.lvs && var_0.l == "var_0";
+
+    //     //var if_end := Block([
+    //     //Ins(ICMP(var_cmp2,ugt,4,var_0,D(Int(0,IntType(4,false))))),
+    //     //Ins(BR(var_cmp2,if_then3(),if_end4()))]);
+
+    //      var if_end4 := Block([Ins(LOAD(var_s,4,var_x)),
+    //                            Ins(CALL(D(Void),printf_code(global_str1()).block)),
+    //                           return_()]);
+
+    //     // var if_then3 := Block([Ins(CALL(D(Void),printf_code(global_str()).block)),
+    //     //                        Ins(UNCONDBR(if_end4()))]);
+    //     var if_then3 := Block([Ins(CALL(D(Void),printf_code(global_str()).block)),
+    //                            if_end4]);
+
+
+    //     var if_end := Block([
+    //     Ins(ICMP(var_cmp2,ugt,4,var_0,D(Int(0,IntType(4,false))))),
+    //     IfElse(var_cmp2,if_then3.block,if_end4.block)]); // fix
+
+    //     if_end
+
+    //     // ASSUMPTIONS (ENGLISH)
+    //     // var_0 has the value of x :: MAX_INT-1 >= x && x < MAX_INT+1
+    // }
+
+    // function benign_vuln_SOI(s:state):codeRe
+    //     requires SOI_ASSIMPTIONS(s)
+    // {
+
+    //      var var_cmp2 := LV(" var_cmp2 ");
+    //     var var_0:operand :| var_0.LV? && var_0.l in s.lvs && var_0.l == "var_0";
+
+    //     var if_end := Block([
+    //     Ins(ICMP(var_cmp2,sgt,4,var_0,D(Int(0,IntType(4,false))))),
+    //     IfElse(var_cmp2,if_then3().block,if_end4().block)]); // fix
+
+    //     if_end
+
+    //     // ASSUMPTIONS (ENGLISH)
+    //     // var_0 has the value of x :: MAX_INT-1 >= x && x < MAX_INT+1
+    // }
+
+
+    function MergedTest(var_x:operand,s:state,patched:bool):codeRe
+        requires SOI_ASSIMPTIONS(s)
+        requires ValidOperand(s,var_x);
+        requires isInt(OperandContents(s,var_x))
+        requires OperandContents(s,var_x).itype.size == 4;
+        requires !OperandContents(s,var_x).itype.signed
+
+        requires OperandContents(s,var_x).val == 2 ==> patched
+        
+    {
+        var var_cmp := LV(" var_cmp ");
+        var var_cmp1 := LV(" var_cmp1 ");
+        var var_cmp2 := LV(" var_cmp2 ");
+        var var_2 := LV(" var_2 ");
+        var var_add := LV(" var_add ");
+                // var var_sub := LV(" var_sub ");
+        var var_sub := D(Int(0,IntType(4,false)));
+                var var_add6 := D(Int(0,IntType(4,false)));
+
+        var var_z := LV(" var_z ");
+        var var_0:operand :| var_0.LV? && var_0.l in s.lvs && var_0.l == "var_0";
+
+        var if_end4 := Block([Ins(SUB(var_sub,4,var_add,D(Int(3,IntType(4,false))))),
+                              Ins(CALL(D(Void),printf_code(Bytes(concatBytes(global_str1().bytes,IntToBytes(var_sub.d)))).block)),
+                              NonImpactIns(ADD(var_add6,4,D(Int(4,IntType(4,false))),D(Int(99,IntType(4,false))))),
+                              NonImpactIns(CALL(D(Void),printf_code(Bytes(concatBytes(global_str2().bytes,IntToBytes(var_add6.d)))).block)),
+                              return_()]);
+
+        var if_then3 := Block([Ins(CALL(D(Void),printf_code(global_str()).block)),
+                               if_end4]);
+
+
+        var if_end := Block([Ins(ADD(var_add,4,var_x,D(Int(2147483646,IntType(4,false))))),
+        Divergence([Ins(ICMP(var_cmp2,sgt,4,var_add,D(Int(0,IntType(4,false)))))], [Ins(ICMP(var_cmp2,ugt,4,var_add,D(Int(0,IntType(4,false)))))],patched),
+        IfElse(var_cmp2,if_then3.block,if_end4.block)]);
+
+        var if_then := Block([return_()]);
+
+
+        // lor.lhs.false:                                    ; preds = %entry
+        //     %cmp1 = icmp sgt i32 %x, 2
+        //     br i1 %cmp1, label %if.then, label %if.end
+
+        var lor_lhs_false :=  Block([Ins(ICMP(var_cmp1,sgt,4,var_x,D(Int(2,IntType(4,false))))),
+                              IfElse(var_cmp1,if_then.block,if_end.block)]);
+
+        // entry:
+        //     %z = alloca i32, align 4
+        //     %cmp = icmp slt i32 %x, 0
+        //     br i1 %cmp, label %if.then, label %lor.lhs.false
+        var entry :=  Block([Ins(ICMP(var_cmp,slt,4,var_x,D(Int(0,IntType(4,false))))),
+                      IfElse(var_cmp,if_then.block,lor_lhs_false.block)]);
+
+        entry
+
+        // ASSUMPTIONS (ENGLISH)
+        // var_0 has the value of x :: MAX_INT-1 >= x && x < MAX_INT+1
+    }
+
+
+
+    predicate SOI_ASSIMPTIONS(s:state)
+    {
+        var var_0 := LV("var_0"); // z
+        ValidState(s)
+        && ValidOperand(s,var_0)
+        && s.o.Nil?
+        && s.lvs["var_0"].Int?
+        && s.lvs["var_0"].val >= 2147483646
+        && s.lvs["var_0"].val <= 2147483648
+        && s.lvs["var_0"].itype.size == 4
+        && !s.lvs["var_0"].itype.signed
+    }
+
+
+
+
+    function global_str():Data
+    {
+       // "z is positive" 
+        var str:Bytes := [0x7a, 0x20, 0x69, 0x73, 0x20, 0x70, 0x6f, 0x73, 0x69, 0x74, 0x69, 0x76, 0x65];
+        Bytes(str)
+    }
+
+    function global_str1():Data
+    {
+       // "done" 
+        var str1:Bytes := [0x64, 0x6f, 0x6e, 0x65];
+        Bytes(str1)
+    }
+
+    function global_str2():Data
+    {
+       // "done" 
+       var str2:Bytes := [0x61, 0x20, 0x3D, 0x0A];
+        // var str2:Bytes := concatBytes([0x61, 0x20, 0x3D, 0x0A], IntToBytes((Int(4,IntType(4,false)))));
+        Bytes(str2)
+    }
+
+
+
+    function printf_code(o:Data):codeRe
+    {
+        Block([Ins(VISIBLE_OUT(Out(o)))])
+    }
+
+}
+
+
+// function benign_vuln_SOI(s:state):codeRe
+//         requires SOI_ASSIMPTIONS(s)
+//     {
+
+//         var var_cmp2 := LV(" var_cmp2 ");
+//         var var_0:operand :| var_0.LV? && var_0.l in s.lvs && var_0.l == "var_0";
+
+//         var return_ := Block([Ins(RET(D(Void)))]);
+
+//         var if_end4 := Block([Ins(CALL(D(Void),printf_code(global_str1()).block)),
+//         Ins(UNCONDBR(return_))]);
+
+//         var if_then3 := Block([Ins(CALL(D(Void),printf_code(global_str()).block)),
+//         Ins(UNCONDBR(if_end4))]);
+
+//         var if_end := Block([
+//         Ins(ICMP(var_cmp2,sgt,4,var_0,D(Int(0,IntType(4,false))))),
+//         Ins(BR(var_cmp2,if_then3,if_end4))]);
+
+//         if_end
+
+//         // ASSUMPTIONS (ENGLISH)
+//         // var_0 has the value of x :: MAX_INT-1 >= x && x < MAX_INT+1
+//     }
